Updates.

HandbookOfPracticalLogicLean/Chapter2/Bool/Semantics.lean
@@ -15,37 +15,55 @@ open Formula_
 
 
 /--
-  A function from the set of atoms to the set of truth values `{False, True}`.
+  A function from the set of atoms to the set of truth values `{false, true}`.
 -/
-def Valuation : Type := String → Prop
+def Valuation : Type := String → Bool
   deriving Inhabited
 
 
+def b_not : Bool → Bool
+| false => true
+| true => false
+
+def b_and : Bool → Bool → Bool
+| false, false => false
+| false, true => false
+| true, false => false
+| true, true => true
+
+def b_or : Bool → Bool → Bool
+| false, false => false
+| false, true => true
+| true, false => true
+| true, true => true
+
+def b_imp : Bool → Bool → Bool
+| false, false => true
+| false, true => true
+| true, false => false
+| true, true => true
+
+def b_iff : Bool → Bool → Bool
+| false, false => true
+| false, true => false
+| true, false => false
+| true, true => true
+
+
 /--
-  `eval V F` := True if and only if the formula `F` evaluates to `True` given the valuation `V`.
+  `eval V F` := The evaluation of a formula `F` given the valuation `V`.
 -/
 def eval
   (V : Valuation) :
-  Formula_ → Prop
-  | false_ => False
-  | true_ => True
+  Formula_ → Bool
+  | false_ => false
+  | true_ => true
   | atom_ X => V X
-  | not_ phi => ¬ eval V phi
-  | and_ phi psi => eval V phi ∧ eval V psi
-  | or_ phi psi => eval V phi ∨ eval V psi
-  | imp_ phi psi => eval V phi → eval V psi
-  | iff_ phi psi => eval V phi ↔ eval V psi
-
-instance
-  (V : Valuation)
-  [DecidablePred V]
-  (F : Formula_) :
-  Decidable (eval V F) :=
-  by
-  induction F
-  all_goals
-    simp only [eval]
-    infer_instance
+  | not_ phi => b_not (eval V phi)
+  | and_ phi psi => b_and (eval V phi) (eval V psi)
+  | or_ phi psi => b_or (eval V phi) (eval V psi)
+  | imp_ phi psi => b_imp (eval V phi) (eval V psi)
+  | iff_ phi psi => b_iff (eval V phi) (eval V psi)
 
 
 /--
@@ -55,11 +73,10 @@ def satisfies
   (V : Valuation)
   (F : Formula_) :
   Prop :=
-  eval V F
+  eval V F = true
 
 instance
   (V : Valuation)
-  [DecidablePred V]
   (F : Formula_) :
   Decidable (satisfies V F) :=
   by
@@ -141,7 +158,13 @@ example
   unfold is_unsatisfiable
   unfold satisfies
   simp only [eval]
-  exact not_exists_not
+  simp only [not_exists]
+  congr!
+  case _ V =>
+    cases eval V F
+    all_goals
+      simp only [b_not]
+      tauto
 
 
 example
@@ -152,7 +175,13 @@ example
   unfold is_tautology
   unfold satisfies
   simp only [eval]
-  exact not_exists
+  simp only [not_exists]
+  congr!
+  case _ V =>
+    cases eval V F
+    all_goals
+      simp only [b_not]
+      tauto
 
 
 example
@@ -172,106 +201,64 @@ example
   unfold is_tautology
   unfold satisfies
   simp only [eval]
+  congr!
+  case _ V =>
+    cases eval V P
+    · cases eval V Q
+      · simp only [b_iff]
+      · simp only [b_iff]
+        tauto
+    · cases eval V Q
+      · simp only [b_iff]
+        tauto
+      · simp only [b_iff]
 
 
 namespace Option_
 
 
-def Valuation : Type := String → Option Prop
+def Valuation : Type := String → Option Bool
   deriving Inhabited
 
 
 def eval
   (V : Valuation) :
-  Formula_ → Option Prop
-  | false_ => some False
-  | true_ => some True
+  Formula_ → Option Bool
+  | false_ => some false
+  | true_ => some true
   | atom_ X => V X
   | not_ phi => do
     let val_phi ← eval V phi
-    ¬ val_phi
+    b_not val_phi
   | and_ phi psi => do
     let val_phi ← eval V phi
     let val_psi ← eval V psi
-    val_phi ∧ val_psi
+    b_and val_phi val_psi
   | or_ phi psi => do
     let val_phi ← eval V phi
     let val_psi ← eval V psi
-    val_phi ∨ val_psi
+    b_or val_phi val_psi
   | imp_ phi psi => do
     let val_phi ← eval V phi
     let val_psi ← eval V psi
-    val_phi → val_psi
+    b_imp val_phi val_psi
   | iff_ phi psi => do
     let val_phi ← eval V phi
     let val_psi ← eval V psi
-    val_phi ↔ val_psi
+    b_iff val_phi val_psi
 
 
-def gen_valuation :
-  List (String × Prop) → Valuation
-  | [] => fun _ => Option.none
-  | hd :: tl => Function.updateITE (gen_valuation tl) hd.fst (Option.some hd.snd)
-
-end Option_
-
---#eval (eval (gen_valuation [("P", True)]) (atom_ "P"))
-
-
-namespace Bool_
-
-
-def b_not : Bool → Bool
-| false => true
-| true => false
-
-def b_and : Bool → Bool → Bool
-| false, false => false
-| false, true => false
-| true, false => false
-| true, true => true
-
-def b_or : Bool → Bool → Bool
-| false, false => false
-| false, true => true
-| true, false => true
-| true, true => true
-
-def b_imp : Bool → Bool → Bool
-| false, false => true
-| false, true => true
-| true, false => false
-| true, true => true
-
-def b_iff : Bool → Bool → Bool
-| false, false => true
-| false, true => false
-| true, false => false
-| true, true => true
-
-
-def Valuation : Type := String → Bool
-  deriving Inhabited
-
-
-def eval
-  (V : Valuation) :
-  Formula_ → Bool
-  | false_ => false
-  | true_ => true
-  | atom_ X => V X
-  | not_ phi => b_not (eval V phi)
-  | and_ phi psi => b_and (eval V phi) (eval V psi)
-  | or_ phi psi => b_or (eval V phi) (eval V psi)
-  | imp_ phi psi => b_imp (eval V phi) (eval V psi)
-  | iff_ phi psi => b_iff (eval V phi) (eval V psi)
-
-
-/-
 def gen_valuation :
   List (String × Bool) → Valuation
   | [] => fun _ => Option.none
   | hd :: tl => Function.updateITE (gen_valuation tl) hd.fst (Option.some hd.snd)
--/
+
+
+#eval (eval (gen_valuation [("P", True)]) (atom_ "P"))
+#eval (eval (gen_valuation [("P", False)]) (atom_ "P"))
+#eval (eval (gen_valuation [("P", True)]) (not_ (atom_ "P")))
+#eval (eval (gen_valuation [("P", False)]) (not_ (atom_ "P")))
+#eval (eval (gen_valuation [("P", True)]) (atom_ "Q"))
+
 
 --#lint
